nola/iris/pborrow_deriv.v
@@ -2,71 +2,44 @@
 
 From nola.util Require Import tagged.
 From nola.bi Require Export deriv.
-From nola.iris Require Export pborrow.
+From nola.iris Require Export pborrow borrow_deriv.
 From iris.proofmode Require Import proofmode.
 Import ProdNotation PlistNotation FunNPNotation iPropAppNotation ModwNotation
   LftNotation ProphNotation DsemNotation.
 
-Implicit Type (TY : synty) (CON : cifcon) (Σ : gFunctors) (FM : ofe).
-
-(** ** [pborrow_judgty]: Judgment type for [pborrow] *)
-Variant pborrow_judg_id TY CON Σ := .
-Definition pborrow_judgty TY CON Σ : ofe := tagged (pborrow_judg_id TY CON Σ)
-  ((** Basic conversion *) cif CON Σ * cif CON Σ +
-  (** Conversion judgment for [lend_body] *)
-    @sigT (TY *' TY) (λ '(X, Y)',
-      leibnizO (clair TY X *' clair TY Y) *
-      (X -d> cif CON Σ) * (Y -d> cif CON Σ)))%type.
-
-(** ** [PborrowJudg]: Judgment structure for [pborrow] *)
-Notation PborrowJudg TY CON Σ JUDG := (Ejudg (pborrow_judgty TY CON Σ) JUDG).
-
 Section pborrow_deriv.
-  Context `{!borrowGS (cifOF CON) Σ, !prophGS TY Σ, !proph_agG TY Σ,
-    pborrow_judg : !PborrowJudg TY CON Σ JUDG}.
+  Context `{!borrowGS (cifOF CON) Σ, !prophGS TY Σ, !proph_agG A TY Σ,
+    !PborrowCon A TY CON, borrow_judg : !BorrowJudg (cifOF CON $oi Σ) JUDG}.
   Implicit Type (δ : JUDG -n> iProp Σ) (Px Qx : cif CON Σ) (X Y : TY).
 
-  (** Judgments *)
-  Local Definition pborrow_jto Px Qx : JUDG :=
-    pborrow_judg (Tagged (inl (Px, Qx))).
-  Local Definition pborrow_jlto {X Y} (xπ : clair TY X) (yπ : clair TY Y)
-    (Φx : X -d> cif CON Σ) (Ψx : Y -d> cif CON Σ) : JUDG :=
-    pborrow_judg (Tagged (inr (existT (X, Y)' ((xπ, yπ)', Φx, Ψx)))).
-  #[export] Instance pborrow_jto_ne : NonExpansive2 pborrow_jto.
-  Proof. solve_proper. Qed.
-  #[export] Instance pborrow_jlto_ne {X Y xπ yπ} :
-    NonExpansive2 (@pborrow_jlto X Y xπ yπ).
-  Proof.
-    unfold pborrow_jlto=> ???????. f_equiv. apply inr_ne. apply: existT_ne=>/=.
-    split; [split|]; solve_proper.
-  Qed.
-
   (** [pbor]: Relaxed prophetic borrower *)
-  Local Definition pbor_def {X} δ α x ξ (Φx : X -d> _) : iProp Σ :=
-    ∃ Ψx, □ (∀ x, δ (pborrow_jto (Φx x) (Ψx x))) ∗
-      □ (∀ x, δ (pborrow_jto (Ψx x) (Φx x))) ∗ pbor_tok α x ξ Ψx.
+  Local Definition pbor_def {X} δ α a xπ ξ (Φx : _ -d> _ -d> cif CON Σ)
+    : iProp Σ :=
+    ∃ Ψx, □ (∀ a xπ, δ (borrow_jto (Φx a xπ) (Ψx a xπ))) ∗
+      □ (∀ a xπ, δ (borrow_jto (Ψx a xπ) (Φx a xπ))) ∗
+      pbor_tok (X:=X) α a xπ ξ Ψx.
   Local Lemma pbor_aux : seal (@pbor_def). Proof. by eexists. Qed.
   Definition pbor {X} := pbor_aux.(unseal) X.
   Local Lemma pbor_unseal : @pbor = @pbor_def. Proof. exact: seal_eq. Qed.
   (** [pobor]: Relaxed prophetic open borrower *)
-  Local Definition pobor_def {X} δ α q ξ (Φx : X -d> _) : iProp Σ :=
-    ∃ Ψx, □ (∀ x, δ (pborrow_jto (Φx x) (Ψx x))) ∗
-      □ (∀ x, δ (pborrow_jto (Ψx x) (Φx x))) ∗ pobor_tok α q ξ Ψx.
+  Local Definition pobor_def {X} δ α q ξ (Φx : _ -d> _ -d> cif CON Σ)
+    : iProp Σ :=
+    ∃ Ψx, □ (∀ a xπ, δ (borrow_jto (Φx a xπ) (Ψx a xπ))) ∗
+      □ (∀ a xπ, δ (borrow_jto (Ψx a xπ) (Φx a xπ))) ∗
+      pobor_tok (X:=X) α q ξ Ψx.
   Local Lemma pobor_aux : seal (@pobor_def). Proof. by eexists. Qed.
   Definition pobor {X} := pobor_aux.(unseal) X.
   Local Lemma pobor_unseal : @pobor = @pobor_def. Proof. exact: seal_eq. Qed.
   (** [plend]: Relaxed prophetic lender *)
-  Local Definition plend_def {X} δ α xπ (Φx : X -d> _) : iProp Σ :=
-    ∃ Y yπ Ψx, □ δ (pborrow_jlto yπ xπ Ψx Φx) ∗ plend_tok (X:=Y) α yπ Ψx.
-  Local Lemma plend_aux : seal (@plend_def). Proof. by eexists. Qed.
-  Definition plend {X} := plend_aux.(unseal) X.
-  Local Lemma plend_unseal : @plend = @plend_def. Proof. exact: seal_eq. Qed.
+  Definition plend {X} δ α xπ (Φx : _ -d> cif CON Σ) : iProp Σ :=
+    lend δ α (cif_xplend (X:=X) xπ Φx).
 
   (** Borrower and lender propositions are non-expansive *)
-  #[export] Instance pbor_ne {δ X α x ξ} : NonExpansive (pbor (X:=X) δ α x ξ).
+  #[export] Instance pbor_ne {δ X α a xπ ξ} :
+    NonExpansive (pbor (X:=X) δ α a xπ ξ).
   Proof. rewrite pbor_unseal. solve_proper. Qed.
-  #[export] Instance pbor_proper {δ X α x ξ} :
-    Proper ((≡) ==> (⊣⊢)) (pbor (X:=X) δ α x ξ).
+  #[export] Instance pbor_proper {δ X α a xπ ξ} :
+    Proper ((≡) ==> (⊣⊢)) (pbor (X:=X) δ α a xπ ξ).
   Proof. apply ne_proper, _. Qed.
   #[export] Instance pobor_ne {δ X α q ξ} : NonExpansive (pobor (X:=X) δ α q ξ).
   Proof. rewrite pobor_unseal. solve_proper. Qed.
@@ -74,7 +47,7 @@ Section pborrow_deriv.
     Proper ((≡) ==> (⊣⊢)) (pobor (X:=X) δ α q ξ).
   Proof. apply ne_proper, _. Qed.
   #[export] Instance plend_ne {δ X α xπ} : NonExpansive (plend (X:=X) δ α xπ).
-  Proof. rewrite plend_unseal. solve_proper. Qed.
+  Proof. solve_proper. Qed.
   #[export] Instance plend_proper {δ X α xπ} :
     Proper ((≡) ==> (⊣⊢)) (plend (X:=X) δ α xπ).
   Proof. apply ne_proper, _. Qed.
@@ -85,133 +58,53 @@ Notation pbord := (pbor der). Notation pobord := (pobor der).
 Notation plendd := (plend der).
 
 Section pborrow_deriv.
-  Context `{!borrowGS (cifOF CON) Σ, !prophGS TY Σ, !proph_agG TY Σ,
-    !PborrowJudg TY CON Σ JUDG, !Jsem JUDG (iProp Σ), !SemCifcon JUDG CON Σ}.
-  Implicit Type (δ : JUDG -n> iProp Σ) (Px Qx : cif CON Σ).
-
-  (** ** [pborrow_judg_sem]: Semantics of [pborrow_judgty] *)
-  Definition pborrow_judg_sem δ (J : pborrow_judgty TY CON Σ) : iProp Σ :=
-    match J.(untag) with
-    | inl PQx => ⟦ PQx.1 ⟧(δ) ==∗ ⟦ PQx.2 ⟧(δ)
-    | inr (existT _ ((xπ, yπ)', Φx, Ψx)) => xplend δ xπ Φx ==∗ xplend δ yπ Ψx
-    end.
-  (** [pborrow_judg_sem] is non-expansive *)
-  #[export] Instance pborrow_judg_sem_ne {δ} :
-    NonExpansive (pborrow_judg_sem δ).
-  Proof.
-    move=> ?[?][?]/=[?|]; [solve_proper|]. move=> [?[[??]?]][?[[??]?]][/=?].
-    subst=>/=. move=> [/=[/=/leibniz_equiv_iff]]. solve_proper.
-  Qed.
-  (** [Dsem] over [pborrow_judgty] *)
-  #[export] Instance pborrow_jto_dsem
-    : Dsem JUDG (pborrow_judgty TY CON Σ) (iProp Σ) :=
-    DSEM pborrow_judg_sem _.
-End pborrow_deriv.
-
-(** ** [PborrowJsem]: Judgment semantics for [pborrow] *)
-Notation PborrowJsem TY CON Σ JUDG :=
-  (Ejsem (pborrow_judgty TY CON Σ) JUDG (iProp Σ)).
-
-Section pborrow_deriv.
-  Context `{!borrowGS (cifOF CON) Σ, !prophGS TY Σ, !proph_agG TY Σ,
-    !PborrowJudg TY CON Σ JUDG, !Jsem JUDG (iProp Σ), !SemCifcon JUDG CON Σ,
-    !PborrowJsem TY CON Σ JUDG, !Deriv (JUDG:=JUDG) ih δ}.
+  Context `{!borrowGS (cifOF CON) Σ, !prophGS TY Σ, !proph_agG A TY Σ,
+    !PborrowCon A TY CON, !BorrowJudg (cifOF CON $oi Σ) JUDG,
+    !Jsem JUDG (iProp Σ), !SemCifcon JUDG CON Σ, !PborrowSem A TY JUDG CON Σ,
+    !BorrowJsem (cifOF CON) Σ JUDG, !Deriv (JUDG:=JUDG) ih δ}.
   Implicit Type (X Y Z : TY) (Px Qx Rx : cif CON Σ) (δ : JUDG -n> iProp Σ).
 
   (** ** Conversion *)
 
-  (** Lemmas for [pborrow_jto] *)
-  Local Lemma pborrow_jto_refl {Px} : ⊢ δ (pborrow_jto Px Px).
-  Proof.
-    iApply Deriv_factor. iIntros (????). rewrite sem_ejudg.
-    by iIntros "$".
-  Qed.
-  Local Lemma pborrow_jto_trans {Px Qx Rx} :
-    (∀ δ', ⌜Deriv ih δ'⌝ → ⌜ih δ'⌝ → ⌜dinto δ δ'⌝ →
-      ⟦ Px ⟧(δ') ==∗ ⟦ Qx ⟧(δ')) -∗
-    δ (pborrow_jto Qx Rx) -∗ δ (pborrow_jto Px Rx).
-  Proof.
-    iIntros "big". iApply Deriv_map. iIntros (????). rewrite !sem_ejudg.
-    iIntros "QR Px". iMod ("big" with "[//] [//] [//] Px"). by iApply "QR".
-  Qed.
-  Local Lemma pborrow_jto_trans' {Px Qx Rx} :
-    (∀ δ', ⌜Deriv ih δ'⌝ → ⌜ih δ'⌝ → ⌜dinto δ δ'⌝ → ⟦ Qx ⟧(δ') ==∗ ⟦ Rx ⟧(δ'))
-      -∗ δ (pborrow_jto Px Qx) -∗ δ (pborrow_jto Px Rx).
-  Proof.
-    iIntros "big". iApply Deriv_map. iIntros (????). rewrite !sem_ejudg.
-    iIntros "PQ Px". iMod ("PQ" with "Px"). by iApply "big".
-  Qed.
-  Local Lemma der_pborrow_jto {Px Qx} :
-    der (pborrow_jto Px Qx) ⊢ (⟦ Px ⟧ ==∗ ⟦ Qx ⟧).
-  Proof. by rewrite der_sound sem_ejudg. Qed.
-
-  (** Lemmas for [pborrow_jlto] *)
-  Local Lemma pborrow_jlto_refl {X xπ Φx} :
-    ⊢ δ (pborrow_jlto (X:=X) xπ xπ Φx Φx).
-  Proof.
-    iApply Deriv_factor. iIntros (????). rewrite sem_ejudg.
-    by iIntros "$".
-  Qed.
-  Local Lemma pborrow_jlto_trans {X Y Z xπ yπ zπ Φx Ψx Ω} :
-    (∀ δ', ⌜Deriv ih δ'⌝ → ⌜ih δ'⌝ → ⌜dinto δ δ'⌝ →
-      xplend δ' xπ Φx ==∗ xplend δ' yπ Ψx) -∗
-    δ (pborrow_jlto (X:=Y) (Y:=Z) yπ zπ Ψx Ω) -∗
-    δ (pborrow_jlto (X:=X) xπ zπ Φx Ω).
-  Proof.
-    iIntros "big". iApply Deriv_map. iIntros (????).
-    rewrite !sem_ejudg. iIntros "ΨΩ Φx".
-    iMod ("big" with "[//] [//] [//] Φx"). by iApply "ΨΩ".
-  Qed.
-  Local Lemma pborrow_jlto_trans' {X Y Z xπ yπ zπ Φx Ψx Ω} :
-    (∀ δ', ⌜Deriv ih δ'⌝ → ⌜ih δ'⌝ → ⌜dinto δ δ'⌝ →
-      xplend δ' yπ Ψx ==∗ xplend δ' zπ Ω) -∗
-    δ (pborrow_jlto (X:=X) (Y:=Y) xπ yπ Φx Ψx) -∗
-    δ (pborrow_jlto (Y:=Z) xπ zπ Φx Ω).
-  Proof.
-    iIntros "big". iApply Deriv_map. iIntros (????).
-    rewrite !sem_ejudg. iIntros "ΦΨ Φx". iMod ("ΦΨ" with "Φx").
-    by iApply "big".
-  Qed.
-  Local Lemma der_pborrow_jlto {X Y xπ yπ Φx Ψx} :
-    der (pborrow_jlto (X:=X) (Y:=Y) xπ yπ Φx Ψx) ⊢
-      (xplendd xπ Φx ==∗ xplendd yπ Ψx).
-  Proof. by rewrite der_sound sem_ejudg. Qed.
+  (** Utility *)
+  Lemma der_borrow_jto' {Px Qx} :
+    der (borrow_jto Px Qx) ⊢ (cif_sem der Px ==∗ cif_sem der Qx).
+  Proof. exact der_borrow_jto. Qed.
 
   (** Convert the body of borrower and lender propositions *)
-  Lemma pbor_to {X α x ξ Φx Ψx} :
-    □ (∀ x' δ', ⌜Deriv ih δ'⌝ → ⌜ih δ'⌝ → ⌜dinto δ δ'⌝ →
-      ⟦ Φx x' ⟧(δ') ==∗ ⟦ Ψx x' ⟧(δ')) -∗
-    □ (∀ x' δ', ⌜Deriv ih δ'⌝ → ⌜ih δ'⌝ → ⌜dinto δ δ'⌝ →
-      ⟦ Ψx x' ⟧(δ') ==∗ ⟦ Φx x' ⟧(δ')) -∗
-    pbor (X:=X) δ α x ξ Φx -∗ pbor δ α x ξ Ψx.
+  Lemma pbor_to {X α a xπ ξ Φx Ψx} :
+    □ (∀ a xπ δ', ⌜Deriv ih δ'⌝ → ⌜ih δ'⌝ → ⌜dinto δ δ'⌝ →
+      ⟦ Φx a xπ ⟧(δ') ==∗ ⟦ Ψx a xπ ⟧(δ')) -∗
+    □ (∀ a xπ δ', ⌜Deriv ih δ'⌝ → ⌜ih δ'⌝ → ⌜dinto δ δ'⌝ →
+      ⟦ Ψx a xπ ⟧(δ') ==∗ ⟦ Φx a xπ ⟧(δ')) -∗
+    pbor (X:=X) δ α a xπ ξ Φx -∗ pbor δ α a xπ ξ Ψx.
   Proof.
     rewrite pbor_unseal. iIntros "#ΦΨ #ΨΦ (%Ω & #ΦΩ & #ΩΦ & $)".
-    iSplit; iIntros (?); [iApply (pborrow_jto_trans with "ΨΦ ΦΩ")|
-      iApply (pborrow_jto_trans' with "ΦΨ ΩΦ")].
+    iSplit; iIntros "!>" (??); [by iApply borrow_jto_trans|].
+    iApply borrow_jto_trans'; by [iApply "ΦΨ"|].
   Qed.
   Lemma pobor_to {X α q ξ Φx Ψx} :
-    □ (∀ x δ', ⌜Deriv ih δ'⌝ → ⌜ih δ'⌝ → ⌜dinto δ δ'⌝ →
-      ⟦ Φx x ⟧(δ') ==∗ ⟦ Ψx x ⟧(δ')) -∗
-    □ (∀ x δ', ⌜Deriv ih δ'⌝ → ⌜ih δ'⌝ → ⌜dinto δ δ'⌝ →
-      ⟦ Ψx x ⟧(δ') ==∗ ⟦ Φx x ⟧(δ')) -∗
+    □ (∀ a xπ δ', ⌜Deriv ih δ'⌝ → ⌜ih δ'⌝ → ⌜dinto δ δ'⌝ →
+      ⟦ Φx a xπ ⟧(δ') ==∗ ⟦ Ψx a xπ ⟧(δ')) -∗
+    □ (∀ a xπ δ', ⌜Deriv ih δ'⌝ → ⌜ih δ'⌝ → ⌜dinto δ δ'⌝ →
+      ⟦ Ψx a xπ ⟧(δ') ==∗ ⟦ Φx a xπ ⟧(δ')) -∗
     pobor (X:=X) δ α q ξ Φx -∗ pobor δ α q ξ Ψx.
   Proof.
     rewrite pobor_unseal. iIntros "#ΦΨ #ΨΦ (%Ω & #ΦΩ & #ΩΦ & $)".
-    iSplit; iIntros (?); [iApply (pborrow_jto_trans with "ΨΦ ΦΩ")|
-      iApply (pborrow_jto_trans' with "ΦΨ ΩΦ")].
+    iSplit; iIntros "!>" (??); [by iApply borrow_jto_trans|].
+    iApply borrow_jto_trans'; by [iApply "ΦΨ"|].
   Qed.
   Lemma plend_to {X Y α xπ yπ Φx Ψx} :
     □ (∀ δ', ⌜Deriv ih δ'⌝ → ⌜ih δ'⌝ → ⌜dinto δ δ'⌝ →
       xplend δ' xπ Φx ==∗ xplend δ' yπ Ψx) -∗
     plend (X:=X) δ α xπ Φx -∗ plend (X:=Y) δ α yπ Ψx.
   Proof.
-    rewrite plend_unseal. iIntros "#ΦΨ (%Z & %zπ & %Ω & #ΩΦ & $)".
-    iApply (pborrow_jlto_trans' with "ΦΨ ΩΦ").
+    iIntros "?". iApply lend_to=>/=. by setoid_rewrite sem_ecustom=>/=.
   Qed.
 
   (** Modify the lifetime of borrower and lender propositions *)
-  Lemma pbor_lft {X α β x ξ Φx} :
-    β ⊑□ α -∗ pbor (X:=X) δ α x ξ Φx -∗ pbor δ β x ξ Φx.
+  Lemma pbor_lft {X α β a xπ ξ Φx} :
+    β ⊑□ α -∗ pbor (X:=X) δ α a xπ ξ Φx -∗ pbor δ β a xπ ξ Φx.
   Proof.
     rewrite pbor_unseal. iIntros "⊑ (% & #? & #? & b)".
     iDestruct (pbor_tok_lft with "⊑ b") as "$". by iSplit.
@@ -224,50 +117,48 @@ Section pborrow_deriv.
   Qed.
   Lemma plend_lft {X α β xπ Φx} :
     α ⊑□ β -∗ plend (X:=X) δ α xπ Φx -∗ plend δ β xπ Φx.
-  Proof.
-    rewrite plend_unseal. iIntros "⊑ (% & % & % & #? & l)".
-    by iDestruct (plend_tok_lft with "⊑ l") as "$".
-  Qed.
+  Proof. exact lend_lft. Qed.
 
   (** Turn from tokens *)
-  Lemma pbor_tok_pbor {X α x ξ Φx} :
-    pbor_tok (X:=X) α x ξ Φx ⊢ pbor δ α x ξ Φx.
+  Lemma pbor_tok_pbor {X α a xπ ξ Φx} :
+    pbor_tok (X:=X) α a xπ ξ Φx ⊢ pbor δ α a xπ ξ Φx.
   Proof.
     rewrite pbor_unseal. iIntros "$".
-    iSplit; iIntros "!> %"; iApply pborrow_jto_refl.
+    iSplit; iIntros "!> %%"; iApply borrow_jto_refl.
   Qed.
   Lemma pobor_tok_pobor {X α q ξ Φx} :
     pobor_tok (X:=X) α q ξ Φx ⊢ pobor δ α q ξ Φx.
   Proof.
     rewrite pobor_unseal. iIntros "$".
-    iSplit; iIntros "!> %"; iApply pborrow_jto_refl.
+    iSplit; iIntros "!> %%"; iApply borrow_jto_refl.
   Qed.
   Lemma plend_tok_plend {X α xπ Φx} :
     plend_tok (X:=X) α xπ Φx ⊢ plend δ α xπ Φx.
-  Proof. rewrite plend_unseal. iIntros "$". iApply pborrow_jlto_refl. Qed.
+  Proof. exact lend_tok_lend. Qed.
 
   Context `{!@ModUpd (iProp Σ) M, !ModBUpd M, !ModExcept0 M}.
 
   (** ** Rules that work under [Deriv ih δ] *)
 
   (** Create new prophetic borrowers and lenders *)
-  Lemma pbor_plend_new_list α Xl (xΦxl : plist _ Xl) :
-    ⊢ |==> ∃ ξl, ∀ Yl (yπΨxl : plist (λ Y, _ *' (Y → _)) Yl),
-      let ξxΦxl := plist_zip ξl xΦxl in
-      ([∗ plist] '(x, Φx)' ∈ xΦxl, ⟦ Φx x ⟧(δ)) -∗
-      ([†α] -∗ ([∗ plist] '(ξ, x, Φx)' ∈ ξxΦxl, xplend_var δ ξ Φx) -∗ M
-        ([∗ plist] '(yπ, Ψx)' ∈ yπΨxl, xplend δ yπ Ψx))
-        =[borrow_wsat M ⟦⟧(δ)]=∗◇
-        ([∗ plist] '(ξ, x, Φx)' ∈ ξxΦxl, pbor δ α x ξ Φx) ∗
+  Lemma pbor_plend_new_list Xl α (axπΦxl : plist _ Xl) :
+    ⊢ |==> ∃ ξl, ∀ Yl (yπΨxl : plist (λ Y, _ *' (clair TY Y → _)) Yl),
+      let ξaxπΦxl := plist_zip ξl axπΦxl in
+      ([∗ plist] '(a, xπ, Φx)' ∈ axπΦxl, ⟦ Φx a xπ ⟧(δ)) -∗
+      ([†α] -∗ ([∗ plist] '(ξ, _, _, Φx)' ∈ ξaxπΦxl,
+        xplend_var δ ξ (λ xπ, ∃ a, Φx a xπ)%cif) -∗
+        M ([∗ plist] '(yπ, Ψx)' ∈ yπΨxl, xplend δ yπ Ψx))
+        =[borrow_wsat M ⟦⟧(δ)]=∗
+        ([∗ plist] '(ξ, a, xπ, Φx)' ∈ ξaxπΦxl, pbor δ α a xπ ξ Φx) ∗
         ([∗ plist] '(yπ, Ψx)' ∈ yπΨxl, plend δ α yπ Ψx).
   Proof.
     simpl. setoid_rewrite <-pbor_tok_pbor. setoid_rewrite <-plend_tok_plend.
     exact: pbor_plend_tok_new_list.
   Qed.
   (** Simply create a prophetic borrower and a prophetic lender *)
-  Lemma pbor_plend_new α X (x : X) Φx :
-    ⟦ Φx x ⟧(δ) =[borrow_wsat M ⟦⟧(δ)]=∗◇ ∃ ξ,
-      pbor δ α x ξ Φx ∗ plend δ α (λ π, π ξ) Φx.
+  Lemma pbor_plend_new X α a xπ Φx :
+    ⟦ Φx a xπ ⟧(δ) =[borrow_wsat M ⟦⟧(δ)]=∗ ∃ ξ,
+      pbor (X:=X) δ α a xπ ξ Φx ∗ plend δ α (λ π, π ξ) (λ xπ, ∃ a, Φx a xπ)%cif.
   Proof.
     setoid_rewrite <-pbor_tok_pbor. setoid_rewrite <-plend_tok_plend.
     exact: pbor_plend_tok_new.
@@ -275,168 +166,133 @@ Section pborrow_deriv.
 End pborrow_deriv.
 
 Section pborrow_deriv.
-  Context `{!borrowGS (cifOF CON) Σ, !prophGS TY Σ, !proph_agG TY Σ,
-    !PborrowJudg TY CON Σ JUDG, !Jsem JUDG (iProp Σ), !SemCifcon JUDG CON Σ,
-    !PborrowJsem TY CON Σ JUDG,
+  Context `{!borrowGS (cifOF CON) Σ, !prophGS TY Σ, !proph_agG A TY Σ,
+    !PborrowCon A TY CON, !BorrowJudg (cifOF CON $oi Σ) JUDG,
+    !Jsem JUDG (iProp Σ), !SemCifcon JUDG CON Σ, !PborrowSem A TY JUDG CON Σ,
+    !BorrowJsem (cifOF CON) Σ JUDG,
     !@ModUpd (iProp Σ) M, !ModBUpd M, !ModExcept0 M}.
   Implicit Type (X Y : TY) (Px Qx : cif CON Σ).
 
   (** Split a prophetic lender *)
-  Lemma plendd_split {X α xπ} {Φx : X → _} Yl
-    (yπΨxl : plist (λ Y, _ *' (Y → _)) Yl) :
+  Lemma plendd_split {X α} {xπ : clair TY X} {Φx} Yl
+    (yπΨxl : plist (λ Y, _ *' (clair TY Y → _)) Yl) :
     plendd α xπ Φx -∗
     (xplendd xπ Φx -∗ M ([∗ plist] '(yπ, Ψx)' ∈ yπΨxl, xplendd yπ Ψx))
-      =[borrow_wsat M ⟦⟧]=∗◇ [∗ plist] '(yπ, Ψx)' ∈ yπΨxl, plendd α yπ Ψx.
+      =[borrow_wsat M ⟦⟧]=∗ [∗ plist] '(yπ, Ψx)' ∈ yπΨxl, plendd α yπ Ψx.
   Proof.
-    rewrite {1}plend_unseal. iIntros "(%Z & %zπ & %Ω & ΩΦ & l) →Ψxl".
-    setoid_rewrite <-plend_tok_plend.
-    iApply (plend_tok_split (M:=M) with "l [ΩΦ →Ψxl]"). iIntros "lb".
-    iMod (der_pborrow_jlto with "ΩΦ lb") as "?". by iApply "→Ψxl".
+    iIntros "/=l →Ψxl".
+    iMod (lendd_split (FML:=cifOF _) (M:=M)
+      (nola.iris.pborrow.cif_xplendl yπΨxl) with "l [→Ψxl]");
+      rewrite big_sepL_of_plist //=.
+    by setoid_rewrite sem_ecustom=>/=.
   Qed.
 
   (** Retrieve from a prophetic lender *)
-  Lemma plendd_retrieve {X α xπ} {Φx : X → _} :
+  Lemma plend_tok_retrieve {X α} {xπ : clair TY X} {Φx} :
     [†α] -∗ plendd α xπ Φx -∗ modw M (borrow_wsat M ⟦⟧) (xplendd xπ Φx).
   Proof.
-    rewrite {1}plend_unseal. iIntros "† (%Y & %yπ & %Ψx & ΨΦ & l)".
-    iMod (plend_tok_retrieve (M:=M) with "† l") as "lb".
-    iMod (der_pborrow_jlto with "ΨΦ lb") as "$". by iIntros.
+    iIntros "† l". iMod (lendd_retrieve with "† l")=>/=.
+    by setoid_rewrite sem_ecustom.
   Qed.
 
   (** Open a prophetic borrower *)
-  Lemma pbord_open {X α q x ξ} {Φx : X → _} :
-    q.[α] -∗ pbord α x ξ Φx -∗ modw M (borrow_wsat M ⟦⟧)
-      (pobord α q ξ Φx ∗ ⟦ Φx x ⟧).
+  Lemma pbord_open {X α q a xπ} {ξ : prvar X} {Φx} :
+    q.[α] -∗ pbord α a xπ ξ Φx -∗ modw M (borrow_wsat M ⟦⟧)
+      (pobord α q ξ Φx ∗ ⟦ Φx a xπ ⟧).
   Proof.
     rewrite pbor_unseal pobor_unseal. iIntros "α (% & $ & #ΨΦ & b)".
     iMod (pbor_tok_open (M:=M) with "α b") as "[$ Ψx]".
-    iMod (der_pborrow_jto with "ΨΦ Ψx") as "$". by iIntros "$".
-  Qed.
-
-  (** Lemma for [pobord_merge_subdiv] *)
-  Local Lemma from_sincl_pobords {Xl A β}
-    {αqξΦxfl : plist (λ X, _ *' _ *' _ *' _ *' (A → X)) Xl} :
-    ([∗ plist] '(α, q, ξ, Φx, _)' ∈ αqξΦxfl, β ⊑□ α ∗ pobord α q ξ Φx) ⊢
-      ∃ αqξΩfl : plist (λ X, _ *' _ *' _ *' _ *' (A → X)) Xl,
-      ⌜([∗ plist] '(α, q, _)' ∈ αqξΦxfl, q.[α]) ⊣⊢
-        [∗ plist] '(α, q, _)' ∈ αqξΩfl, q.[α]⌝ ∗
-      ⌜∀ aπ,
-        ([∗ plist] '(_, _, ξ, _, f)' ∈ αqξΦxfl,
-          ⟨π, π (Aprvar _ ξ) = f (aπ π)⟩) ⊣⊢
-        [∗ plist] '(_, _, ξ, _, f)' ∈ αqξΩfl, ⟨π, π (Aprvar _ ξ) = f (aπ π)⟩⌝ ∗
-      ([∗ plist] '(α, q, ξ, Ω, _)' ∈ αqξΩfl, β ⊑□ α ∗ pobor_tok α q ξ Ω) ∗
-      (∀ a, ([∗ plist] '(_, _, _, Φx, f)' ∈ αqξΦxfl, ⟦ Φx (f a) ⟧) ==∗
-        [∗ plist] '(_, _, _, Ω, f)' ∈ αqξΩfl, ⟦ Ω (f a) ⟧).
-  Proof.
-    rewrite pobor_unseal. elim: Xl αqξΦxfl=>/=.
-    { iIntros. iExists (). do 2 (iSplit; [done|]). by iIntros. }
-    move=> X Xl IH [[α[q[ξ[Φx f]]]] αqξΦxfl]. rewrite IH.
-    iIntros "[[⊑ (%Ω & #ΦΩ & _ & o)] [%αqξΩfl[%[%[ol →']]]]]".
-    iExists ((α, q, ξ, Ω, f)', αqξΩfl)'. iFrame "⊑ o ol".
-    do 2 (iSplit; [iPureIntro=> >; by f_equiv|]). iIntros (a) "[Φx Φxl]".
-    iMod (der_pborrow_jto with "ΦΩ Φx") as "$". by iApply "→'".
-  Qed.
-  (** Merge and subdivide prophetic borrowers *)
-  Lemma pobord_merge_subdiv Xl Yl
-    (αqξΦxfl : plist (λ X, _ *' _ *' _ *' _ *' (_ → X)) Xl) (yΨxl : plist _ Yl)
-    Rxl β :
-    ([∗ plist] '(α, q, ξ, Φx, _)' ∈ αqξΦxfl, β ⊑□ α ∗ pobord α q ξ Φx) -∗
-    ([∗ plist] '(y, Ψx)' ∈ yΨxl, ⟦ Ψx y ⟧) -∗ ([∗ list] Rx ∈ Rxl, ⟦ Rx ⟧) -∗
-    (∀ yl', [†β] -∗ ([∗ plist] '(y', _, Ψx)' ∈ plist_zip yl' yΨxl, ⟦ Ψx y' ⟧) -∗
-      ([∗ list] Rx ∈ Rxl, ⟦ Rx ⟧) -∗ M
-        ([∗ plist] '(_, _, _, Φx, f)' ∈ αqξΦxfl, ⟦ Φx (f yl') ⟧))
-      =[borrow_wsat M ⟦⟧]=∗◇ ∃ ηl,
-      ([∗ plist] '(α, q, _)' ∈ αqξΦxfl, q.[α]) ∗
-      ([∗ plist] '(_, _, ξ, _, f)' ∈ αqξΦxfl,
-        ⟨π, π (Aprvar _ ξ) = f (app_plist_prvar π ηl)⟩) ∗
-      ([∗ plist] '(η, y, Ψx)' ∈ plist_zip ηl yΨxl, pbord β y η Ψx) ∗
-      [∗ list] Rx ∈ Rxl, bor_tok β Rx.
-  Proof.
-    rewrite from_sincl_pobords /=.
-    iIntros "(% & %eq & %eq' & ol & →) Ψxl Rxl →Φxl". setoid_rewrite eq.
-    setoid_rewrite eq'. setoid_rewrite <-pbor_tok_pbor.
-    iApply (pobor_tok_merge_subdiv (M:=M) with "ol Ψxl Rxl").
-    iIntros "% † Ψxl Rxl". iMod ("→Φxl" with "† Ψxl Rxl") as "Φxl".
-    by iMod ("→" with "Φxl").
-  Qed.
-  (** Subdivide a prophetic borrower *)
-  Lemma pobord_subdiv {X α q ξ Φx} Yl (f : _ → X) (yΨxl : plist _ Yl) Rxl β :
-    β ⊑□ α -∗ pobord α q ξ Φx -∗
-    ([∗ plist] '(y, Ψx)' ∈ yΨxl, ⟦ Ψx y ⟧) -∗ ([∗ list] Rx ∈ Rxl, ⟦ Rx ⟧) -∗
-    (∀ yl', [†β] -∗ ([∗ plist] '(y', _, Ψx)' ∈ plist_zip yl' yΨxl, ⟦ Ψx y' ⟧) -∗
-      ([∗ list] Rx ∈ Rxl, ⟦ Rx ⟧) -∗ M ⟦ Φx (f yl') ⟧) =[borrow_wsat M ⟦⟧]=∗◇
-      ∃ ηl,
-      q.[α] ∗ ⟨π, π (Aprvar _ ξ) = f (app_plist_prvar π ηl)⟩ ∗
-      ([∗ plist] '(η, y, Ψx)' ∈ plist_zip ηl yΨxl, pbord β y η Ψx) ∗
-      [∗ list] Rx ∈ Rxl, bor_tok β Rx.
-  Proof.
-    iIntros "⊑ o Ψxl Rxl →Φx".
-    iMod (pobord_merge_subdiv [_] _ ((_,_,_,_,_)',())'
-      with "[$⊑ $o //] Ψxl Rxl [→Φx]") as (?) "/=[[$ _][[$ _]$]]"; [|done].
-    iIntros (?). by rewrite /= bi.sep_emp.
-  Qed.
-
-  (** Resolve the prophecy of a prophetic borrower *)
-  Lemma pobord_resolve {X α q ξ Φx} (x : X) :
-    pobord α q ξ Φx -∗ ⟦ Φx x ⟧ =[borrow_wsat M ⟦⟧]=∗◇
-      q.[α] ∗ ⟨π, π ξ = x⟩ ∗ bor_tok α (Φx x).
-  Proof.
-    iIntros "o Φx".
-    iMod (pobord_subdiv [] (λ _, x) () [Φx x] with "[] o [//] [Φx] []")
-      as (?) "[$[$[_[$ _]]]]"=>/=;
-      by [iApply lft_sincl_refl|iFrame|iIntros "% _ _ [$ _]"|].
-  Qed.
-  Lemma pbord_resolve {X α q x ξ} {Φx : X → _} :
-    q.[α] -∗ pbord α x ξ Φx -∗ modw M (borrow_wsat M ⟦⟧)
-      (q.[α] ∗ ⟨π, π ξ = x⟩ ∗ bor_tok α (Φx x)).
-  Proof.
-    iIntros "α b". iMod (pbord_open with "α b") as "[o Φx]".
-    iMod (pobord_resolve with "o Φx") as "$". by iIntros.
+    iMod (der_borrow_jto with "ΨΦ Ψx") as "$". by iIntros "$".
   Qed.
 
   (** Subdivide a prophetic borrower without changing the prophecy *)
-  Lemma pobord_nsubdiv {X α q ξ Φx} Ψx (x : X) β :
-    β ⊑□ α -∗ pobord α q ξ Φx -∗ ⟦ Ψx x ⟧ -∗
-    (∀ x', [†β] -∗ ⟦ Ψx x' ⟧ -∗ M ⟦ Φx x' ⟧) =[borrow_wsat M ⟦⟧]=∗
-      q.[α] ∗ pbord β x ξ Ψx.
+  Lemma pobord_nsubdiv {X α q ξ Φx} Ψx a (xπ : clair TY X) β :
+    β ⊑□ α -∗ pobord α q ξ Φx -∗ ⟦ Ψx a xπ ⟧ -∗
+    (∀ a' xπ', [†β] -∗ ⟦ Ψx a' xπ' ⟧ -∗ M ⟦ Φx a' xπ' ⟧)
+      =[borrow_wsat M ⟦⟧]=∗ q.[α] ∗ pbord β a xπ ξ Ψx.
   Proof.
     rewrite pobor_unseal. iIntros "⊑ (%Ω & #ΦΩ & _ & o) Ψx →Φx".
     rewrite -pbor_tok_pbor.
     iApply (pobor_tok_nsubdiv (M:=M) with "⊑ o Ψx [ΦΩ →Φx]").
-    iIntros "% † Ψx". iMod ("→Φx" with "† Ψx") as "Φx".
-    by iMod (der_pborrow_jto with "ΦΩ Φx").
+    iIntros "%% † Ψx". iMod ("→Φx" with "† Ψx") as "Φx".
+    by iMod (der_borrow_jto with "ΦΩ Φx").
   Qed.
   (** Simply close a prophetic borrower *)
-  Lemma pobord_close {X α q ξ Φx} (x : X) :
-    pobord α q ξ Φx -∗ ⟦ Φx x ⟧ =[borrow_wsat M ⟦⟧]=∗ q.[α] ∗ pbord α x ξ Φx.
+  Lemma pobord_close {X α q ξ Φx} a (xπ : clair TY X) :
+    pobord α q ξ Φx -∗ ⟦ Φx a xπ ⟧ =[borrow_wsat M ⟦⟧]=∗
+      q.[α] ∗ pbord α a xπ ξ Φx.
   Proof.
     iIntros "o Φx". iApply (pobord_nsubdiv Φx with "[] o Φx"); [|by iIntros].
     iApply lft_sincl_refl.
   Qed.
 
-  (** Reborrow a nested prophetic borrower *)
-  Lemma pobord_pobord_reborrow {X Y α q ξ Φx β r η Ψx} y (f : X → Y) :
-    β ⊑□ α -∗ pobord β q ξ Φx -∗ pobord α r η Ψx -∗ ⟦ Ψx y ⟧ -∗
-    (∀ y', [†β] -∗ pbord α y' η Ψx -∗ M ⟦ Φx (f y') ⟧) -∗
-      modw M (borrow_wsat M ⟦⟧) (∃ η',
-      q.[β] ∗ r.[α] ∗ ⟨π, π ξ = f (π (Aprvar _ η'))⟩ ∗ pbord β y η' Ψx).
+  (** Subdivide a prophetic borrower *)
+  Lemma pobord_subdiv {X α q r ξ Φx}
+    Yl (fπ : clair TY (_ → X)) ζl (ayπΨxl : plist _ Yl) Rxl β :
+    (∀ π π' p p', fπ π p = fπ π' p' → p = p') →
+    (∀ p, proph_dep (λ π, fπ π p) ζl) →
+    pobord α q ξ Φx =[r:∗[ζl]]=∗ ∃ ηl,
+      ⟨π, π (Aprvar _ ξ) = fπ π (app_plist_prvar π ηl)⟩ ∗
+      (β ⊑□ α -∗
+        ([∗ plist] '(a, yπ, Ψx)' ∈ ayπΨxl, ⟦ Ψx a yπ ⟧) -∗
+        ([∗ list] Rx ∈ Rxl, ⟦ Rx ⟧) -∗
+        (∀ yπl', [†β] -∗
+          ([∗ plist] '(yπ', _, _, Ψx)' ∈ plist_zip yπl' ayπΨxl,
+            ⟦ ∃ a, Ψx a yπ' ⟧%cif) -∗
+          ([∗ list] Rx ∈ Rxl, ⟦ Rx ⟧) -∗
+            M ⟦ ∃ a, Φx a (λ π, fπ π (app_plist_clair π yπl')) ⟧%cif)
+          =[borrow_wsat M ⟦⟧]=∗
+          q.[α] ∗
+          ([∗ plist] '(η, a, yπ, Ψx)' ∈ plist_zip ηl ayπΨxl,
+            pbord β a yπ η Ψx) ∗
+          [∗ list] Rx ∈ Rxl, bord β Rx).
   Proof.
-    rewrite pobor_unseal pbor_unseal.
-    iIntros "⊑ (%Φx' & #ΦΦ' & #Φ'Φ & o) (%Ψx' & #ΨΨ' & #Ψ'Ψ & o') Ψx →Φx".
-    iMod (der_pborrow_jto with "ΨΨ' Ψx") as "Ψx'".
-    iMod (pobor_pobor_tok_reborrow (M:=M)
-      with "⊑ o o' Ψx' [→Φx]") as (?) "($ & $ & obs & b)"; last first.
-    { iIntros "$ !>". iFrame "obs b". by iSplit. }
-    iIntros "% † b". iMod ("→Φx" with "† [$b]") as "Φx"; [by iSplit|].
-    by iMod (der_pborrow_jto with "ΦΦ' Φx").
+    rewrite pobor_unseal=> ??. iIntros "(%Φx' & #ΦΦ' & #? & o)".
+    iMod (pobor_tok_subdiv with "o") as (?) "[$ big]"; [done..|].
+    iIntros "!> ⊑ Ψxl Rxl →Φx". setoid_rewrite <-pbor_tok_pbor.
+    setoid_rewrite <-bor_tok_bor. iApply ("big" with "⊑ Ψxl Rxl").
+    iIntros "% † Ψxl Rxl". iMod ("→Φx" with "† Ψxl Rxl") as "/=[% Φx]".
+    by iMod (der_borrow_jto' with "ΦΦ' Φx") as "$".
   Qed.
-  Lemma pobord_pbord_reborrow {X Y α q ξ Φx β r y η Ψx} (f : X → Y) :
-    β ⊑□ α -∗ pobord β q ξ Φx -∗ r.[α] -∗ pbord α y η Ψx -∗
-    (∀ y', [†β] -∗ pbord α y' η Ψx -∗ M ⟦ Φx (f y') ⟧) -∗
-      modw M (borrow_wsat M ⟦⟧) (∃ η',
-        q.[β] ∗ r.[α] ∗ ⟨π, π ξ = f (π (Aprvar _ η'))⟩ ∗ pbord β y η' Ψx).
+
+  (** Resolve the prophecy of a prophetic borrower *)
+  Lemma pobord_resolve {X α q r ξ Φx} a (xπ : clair TY X) ηl :
+    proph_dep xπ ηl →
+    pobord α q ξ Φx =[r:∗[ηl]]=∗
+      ⟨π, π ξ = xπ π⟩ ∗
+      (⟦ Φx a xπ ⟧ =[borrow_wsat M ⟦⟧]=∗ q.[α] ∗ bord α (Φx a xπ)).
   Proof.
-    iIntros "⊑ o r b →Φx". iMod (pbord_open with "r b") as "[o' Ψx]".
-    iApply (pobord_pobord_reborrow with "⊑ o o' Ψx →Φx").
+    iIntros (?) "o".
+    iMod (pobord_subdiv [] (λ π _, xπ π) ηl () [Φx a xπ] with "o")
+      as "[%[$ big]]"=>//=. { by move=> ??[][]. }
+    iIntros "!> Φx".
+    iMod ("big" with "[] [//] [$Φx //] []") as "($ & _ & $ & _)"=>//.
+    { iApply lft_sincl_refl. } { by iIntros "_ _ _ [$ _]". }
+  Qed.
+
+  (** Reborrow a nested prophetic borrower *)
+  Lemma pobord_pbord_reborrow {X Y α q ξ Φx β r η Ψx a yπ}
+    (fπ : clair TY (Y → X)) :
+    (∀ π π' y y', fπ π y = fπ π' y' → y = y') →
+    β ⊑□ α -∗ r.[α] -∗
+    pobord β q ξ Φx -∗ pbord α a yπ η Ψx -∗
+    (∀ a' yπ', [†β] -∗ pbord α a' yπ' η Ψx -∗ M
+      ⟦ Φx a' (λ π, fπ π (yπ' π)) ⟧) -∗
+      modw M (borrow_wsat M ⟦⟧) (1:[η] ∗ ⟦ Ψx a yπ ⟧ ∗
+        ∀ ζl s, ⌜∀ y, proph_dep (λ π, fπ π y) ζl⌝ -∗ s:∗[ζl]
+          ==∗ ∃ η' : prvar _, ⟨π, π ξ = fπ π (π η')⟩ ∗ s:∗[ζl] ∗
+            (1:[η] -∗ ⟦ Ψx a yπ ⟧ =[borrow_wsat M ⟦⟧]=∗
+              q.[β] ∗ r.[α] ∗ pbord β a yπ η' Ψx)).
+  Proof.
+    rewrite pobor_unseal pbor_unseal. iIntros (?) "⊑ α".
+    iIntros "(%Φx' & #ΦΦ' & #? & o) (%Ψx' & #ΨΨ' & #Ψ'Ψ & b) →Φx".
+    iMod (pobor_pbor_tok_reborrow with "⊑ α o b [→Φx]") as "($ & Ψ'x & big)".
+    { done. }
+    { iIntros "%% † b". iMod ("→Φx" with "† [$b]") as "Φx"; [by iSplit|].
+      by iMod (der_borrow_jto with "ΦΦ' Φx"). }
+    iMod (der_borrow_jto with "Ψ'Ψ Ψ'x") as "$". iModIntro.
+    iIntros (???) "ζl". iMod ("big" with "[//] ζl") as (?) "($ & $ & big)".
+    iIntros "!> η Ψx". iMod (der_borrow_jto with "ΨΨ' Ψx") as "Ψx'".
+    iMod ("big" with "η Ψx'") as "($ & $ & $)". iModIntro. by iSplit.
   Qed.
 End pborrow_deriv.
