nola/iris/proph_ag.v
@@ -2,162 +2,152 @@
 
 From nola.iris Require Export proph.
 From nola.util Require Import prod.
+From nola.bi Require Import modw.
 From iris.bi Require Import fractional.
 From iris.base_logic.lib Require Import ghost_var.
 From iris.proofmode Require Import proofmode.
-Import ProphNotation.
+Import ProdNotation ProphNotation ModwNotation.
 
-Implicit Type TY : synty.
+Implicit Type (A : Type) (TY : synty).
 
 (** Ghost state *)
-Class proph_agG TY Σ := proph_agG_in :: ghost_varG Σ (sigT' (@id TY)).
-Definition proph_agΣ TY := ghost_varΣ (sigT' (@id TY)).
-#[export] Instance subG_proph_agΣ `{!subG (proph_agΣ TY) Σ} : proph_agG TY Σ.
+Class proph_agG A TY Σ :=
+  proph_agG_in :: ghost_varG Σ (A *' sigT' (λ X : TY, clair TY X)).
+Definition proph_agΣ A TY := ghost_varΣ (A *' sigT' (λ X : TY, clair TY X)).
+#[export] Instance subG_proph_agΣ `{!subG (proph_agΣ A TY) Σ} :
+  proph_agG A TY Σ.
 Proof. solve_inG. Qed.
 
 Implicit Type γ : gname.
 Section proph_ag.
-  Context `{!proph_agG TY Σ, !prophGS TY Σ}.
+  Context `{!proph_agG A TY Σ, !prophGS TY Σ}.
   Implicit Type X : TY.
 
   (** Value observer *)
-  Local Definition val_obs_def {X} γ x : iProp Σ :=
-    ghost_var γ (1/2) (existT' X x).
+  Local Definition val_obs_def {X} γ a xπ : iProp Σ :=
+    ghost_var γ (1/2) (a, existT' X xπ)'.
   Local Lemma val_obs_aux : seal (@val_obs_def). Proof. by eexists. Qed.
   Definition val_obs {X} := val_obs_aux.(unseal) X.
   Local Lemma val_obs_unseal : @val_obs = @val_obs_def.
   Proof. exact: seal_eq. Qed.
 
   (** Double value observer *)
-  Local Definition val_obs2 {X} γ x : iProp Σ := ghost_var γ 1 (existT' X x).
+  Local Definition val_obs2 {X} γ a xπ : iProp Σ :=
+    ghost_var γ 1 (a, existT' X xπ)'.
 
   (** Prophecy controller *)
-  Local Definition proph_ctrl_def {X} γ x (ξ : prvar X) : iProp Σ :=
-    (val_obs γ x ∗ 1:[ξ]) ∨
-    ((∃ x' : X, val_obs2 γ x') ∗ ⟨π, π ξ = x⟩).
+  Local Definition proph_ctrl_def {X} γ a xπ (ξ : prvar X) : iProp Σ :=
+    (val_obs γ a xπ ∗ 1:[ξ]) ∨
+      ((∃ a' xπ', @val_obs2 X γ a' xπ') ∗ proph_eqz (λ π, π ξ) xπ).
   Local Lemma proph_ctrl_aux : seal (@proph_ctrl_def). Proof. by eexists. Qed.
   Definition proph_ctrl {X} := proph_ctrl_aux.(unseal) X.
   Local Lemma proph_ctrl_unseal : @proph_ctrl = @proph_ctrl_def.
   Proof. exact: seal_eq. Qed.
 
-  (** [val_obs] and [proph_ctrl] are timeless *)
-  #[export] Instance val_obs_timeless {X γ x} : Timeless (val_obs (X:=X) γ x).
+  (** [val_obs] is timeless *)
+  #[export] Instance val_obs_timeless {X γ a xπ} : Timeless (@val_obs X γ a xπ).
   Proof. rewrite val_obs_unseal. exact _. Qed.
-  #[export] Instance proph_ctrl_timeless {X γ x ξ} :
-    Timeless (proph_ctrl (X:=X) γ x ξ).
-  Proof. rewrite proph_ctrl_unseal. exact _. Qed.
 
   (** Allocate two [val_obs]s *)
-  Lemma vo_vo_alloc {X x} :
-    ⊢ |==> ∃ γ, val_obs (X:=X) γ x ∗ val_obs γ x.
+  Lemma vo_vo_alloc {X a xπ} : ⊢ |==> ∃ γ, @val_obs X γ a xπ ∗ val_obs γ a xπ.
   Proof.
     rewrite val_obs_unseal. iMod ghost_var_alloc as (γ) "[??]". iExists _.
     by iFrame.
   Qed.
 
   (** Agreement between two [val_obs]s *)
-  Lemma vo_vo_agree {X γ x x'} :
-    val_obs (X:=X) γ x -∗ val_obs γ x' -∗ ⌜x = x'⌝.
+  Lemma vo_vo_agree {X γ a xπ a' xπ'} :
+    @val_obs X γ a xπ -∗ val_obs γ a' xπ' -∗ ⌜a = a' ∧ xπ = xπ'⌝.
   Proof.
     rewrite val_obs_unseal. iIntros "vo vo'".
     iDestruct (ghost_var_agree with "vo vo'") as %?. by simplify_eq.
   Qed.
 
   (** Update the value of two [val_obs]s *)
-  Lemma vo_vo_update {X γ x x' y} :
-    val_obs (X:=X) γ x -∗ val_obs (X:=X) γ x' ==∗
-      val_obs (X:=X) γ y ∗ val_obs γ y.
+  Lemma vo_vo_update {X γ a xπ a' xπ' a'' xπ''} :
+    @val_obs X γ a xπ -∗ @val_obs X γ a' xπ' ==∗
+      @val_obs X γ a'' xπ'' ∗ val_obs γ a'' xπ''.
   Proof.
     rewrite val_obs_unseal. iIntros "vo vo'".
-    iApply (ghost_var_update_2 with "vo vo'"). by rewrite Qp.div_2.
+    iApply (ghost_var_update_2 with "vo vo'"). apply Qp.div_2.
   Qed.
 
-  (** Get [proph_ctrl] out of [val_obs] and a prophecy token *)
-  Lemma vo_proph_pc {X γ x ξ} :
-    ⊢ val_obs (X:=X) γ x -∗ 1:[Aprvar _ ξ] -∗ proph_ctrl γ x ξ.
-  Proof.
-    rewrite proph_ctrl_unseal. iIntros "vo ξ". iLeft. iFrame.
-  Qed.
+  (** Construct [proph_ctrl] out of [val_obs] and a prophecy token *)
+  Lemma vo_proph_pc {X γ a xπ ξ} :
+    @val_obs X γ a xπ -∗ 1:[Aprvar _ ξ] -∗ proph_ctrl γ a xπ ξ.
+  Proof. rewrite proph_ctrl_unseal. iIntros "vo ξ". iLeft. iFrame. Qed.
 
   (** Allocate [val_obs] and [proph_ctrl] *)
-  Lemma vo_pc_alloc {X x} {ξ : prvar X} :
-    1:[ξ] ==∗ ∃ γ, val_obs γ x ∗ proph_ctrl γ x ξ.
+  Lemma vo_pc_alloc {X a xπ} {ξ : prvar X} :
+    1:[ξ] ==∗ ∃ γ, val_obs γ a xπ ∗ proph_ctrl γ a xπ ξ.
   Proof.
     iIntros "ξ". iMod vo_vo_alloc as (γ) "[vo vo']". iModIntro. iExists _.
     iFrame "vo". iApply (vo_proph_pc with "vo' ξ").
   Qed.
 
   (** Turn two [val_obs] into [val_obs2] *)
-  Local Lemma vo_vo_vo2 {X γ x x'} :
-    val_obs (X:=X) γ x -∗ val_obs (X:=X) γ x' -∗ val_obs2 γ x.
+  Local Lemma vo_vo_vo2 {X γ a xπ a' xπ'} :
+    @val_obs X γ a xπ -∗ @val_obs X γ a' xπ' -∗ val_obs2 γ a xπ.
   Proof.
     rewrite val_obs_unseal. iIntros "vo vo'". iCombine ("vo vo'") as "$".
   Qed.
 
   (** [val_obs] and [val_obs2] can't co-exist *)
-  Local Lemma vo_vo2_no {X γ x x'} :
-    val_obs (X:=X) γ x -∗ val_obs2 (X:=X) γ x' -∗ False.
+  Local Lemma vo_vo2_no {X γ a xπ a' xπ'} :
+    @val_obs X γ a xπ -∗ val_obs2 (X:=X) γ a' xπ' -∗ False.
   Proof.
     rewrite val_obs_unseal. iIntros "vo vo2".
     by iDestruct (ghost_var_valid_2 with "vo vo2") as %[? _].
   Qed.
 
-  (** Agreement between [val_obs] and [proph_ctrl] *)
-  Lemma vo_pc_agree {X γ x x' ξ} :
-    val_obs (X:=X) γ x -∗ proph_ctrl γ x' ξ -∗ ⌜x = x'⌝.
+  (** Turn [proph_ctrl] into a prophecy equalizer *)
+  Lemma pc_eqz {X γ a xπ ξ} :
+    proph_ctrl (X:=X) γ a xπ ξ ⊢ proph_eqz (λ π, π ξ) xπ.
   Proof.
-    rewrite proph_ctrl_unseal. iIntros "vo [[vo' _]|[[% vo2]_]]".
+    rewrite proph_ctrl_unseal. iIntros "[[_ ξ]|[_ $]]".
+    iApply (proph_eqz_tok with "ξ").
+  Qed.
+
+  (** Agreement between [val_obs] and [proph_ctrl] *)
+  Lemma vo_pc_agree {X γ a xπ a' xπ' ξ} :
+    @val_obs X γ a xπ -∗ proph_ctrl γ a' xπ' ξ -∗ ⌜a = a' ∧ xπ = xπ'⌝.
+  Proof.
+    rewrite proph_ctrl_unseal. iIntros "vo [[vo' _]|[(% & % & vo2) _]]".
     - iApply (vo_vo_agree with "vo vo'").
     - iDestruct (vo_vo2_no with "vo vo2") as %[].
   Qed.
 
   (** Turn [proph_ctrl] into [val_obs] and a prophecy token under [val_obs] *)
-  Lemma vo_pc_vo_proph {X γ x x' ξ} :
-    ⊢ val_obs (X:=X) γ x -∗ proph_ctrl (X:=X) γ x' ξ -∗
-      val_obs γ x ∗ val_obs γ x ∗ 1:[Aprvar _ ξ].
+  Lemma vo_pc_proph {X γ a xπ a' xπ' ξ} :
+    @val_obs X γ a xπ -∗ proph_ctrl (X:=X) γ a' xπ' ξ -∗
+      val_obs γ a xπ ∗ val_obs γ a' xπ' ∗ 1:[Aprvar _ ξ].
   Proof.
-    iIntros "vo pc". iDestruct (vo_pc_agree with "vo pc") as %<-.
-    rewrite proph_ctrl_unseal. iDestruct "pc" as "[$|[[% vo2]_]]"; [done|].
+    rewrite proph_ctrl_unseal. iIntros "vo [$|[(% & % & vo2) _]]"; [done|].
     iDestruct (vo_vo2_no with "vo vo2") as %[].
   Qed.
 
   (** Update the value of [val_obs] and [proph_ctrl] *)
-  Lemma vo_pc_update {X γ x x' y ξ} :
-    val_obs (X:=X) γ x -∗ proph_ctrl γ x' ξ ==∗
-      val_obs (X:=X) γ y ∗ proph_ctrl γ y ξ.
+  Lemma vo_pc_update {X γ a xπ a' xπ' a'' xπ'' ξ} :
+    @val_obs X γ a xπ -∗ proph_ctrl γ a' xπ' ξ ==∗
+      @val_obs X γ a'' xπ'' ∗ proph_ctrl γ a'' xπ'' ξ.
   Proof.
-    iIntros "vo pc". iDestruct (vo_pc_vo_proph with "vo pc") as "[vo[vo' ξ]]".
+    iIntros "vo pc". iDestruct (vo_pc_proph with "vo pc") as "[vo [vo' ξ]]".
     iMod (vo_vo_update with "vo vo'") as "[$ vo']". iModIntro.
     iApply (vo_proph_pc with "vo' ξ").
   Qed.
 
-  (** Resolve the prophecy of [proph_ctrl] with [val_obs],
-    retaining [proph_ctrl] *)
-  Lemma vo_pc_preresolve {X γ x x' ξ} aπ ηl q : proph_dep aπ ηl →
-    q:∗[ηl] -∗ val_obs (X:=X) γ x -∗ proph_ctrl (X:=X) γ x' ξ ==∗
-      q:∗[ηl] ∗ ⟨π, π ξ = aπ π⟩ ∗
-      (∀ x'', ⟨π, aπ π = x''⟩ -∗ proph_ctrl γ x'' ξ).
+  (** Resolve the prophecy of [proph_ctrl] with [val_obs], retaining
+    [proph_ctrl] *)
+  Lemma vo_pc_preresolve {X γ a0 xπ0 a1 xπ1 ξ} xπ ηl q :
+    proph_dep xπ ηl →
+    @val_obs X γ a0 xπ0 -∗ proph_ctrl (X:=X) γ a1 xπ1 ξ =[q:∗[ηl]]=∗
+      ⟨π, π ξ = xπ π⟩ ∗ (∀ a' xπ', proph_eqz xπ xπ' -∗ proph_ctrl γ a' xπ' ξ).
   Proof.
-    iIntros "% ηl vo pc".
-    iDestruct (vo_pc_vo_proph with "vo pc") as "[vo[vo' ξ]]".
+    iIntros "% vo pc ηl".
+    iDestruct (vo_pc_proph with "vo pc") as "(vo & vo' & ξ)".
     iMod (proph_resolve_dep with "ξ ηl") as "[$ #obs]"; [done|]. iModIntro.
-    iFrame "obs". iIntros "%y obs'". rewrite proph_ctrl_unseal. iRight.
-    iDestruct (vo_vo_vo2 with "vo vo'") as "vo2". iSplit; [by iExists _|].
-    by iApply (proph_obs_impl2 with "obs obs'")=> ?->.
-  Qed.
-  Lemma vo_pc_resolve {X γ} {x x' x'' : X} {ξ} :
-    val_obs (X:=X) γ x -∗ proph_ctrl γ x' ξ ==∗
-      ⟨π, π ξ = x''⟩ ∗ proph_ctrl γ x'' ξ.
-  Proof.
-    iIntros "vo pc".
-    iMod (vo_pc_preresolve (λ _, x'') [] 1 with "[//] vo pc") as "[_[$ →pc]]".
-    { done. } iModIntro. iApply "→pc". by iApply proph_obs_true.
-  Qed.
-
-  (** Resolve the prophecy of [proph_ctrl] *)
-  Lemma pc_resolve {X γ x} ξ : proph_ctrl (X:=X) γ x ξ ==∗ ⟨π, π ξ = x⟩.
-  Proof.
-    rewrite proph_ctrl_unseal. iIntros "[[_ ξ]|[_ $]]"; [|done].
-    iApply (proph_resolve with "ξ").
+    iFrame "obs". iIntros "% % eqz". rewrite proph_ctrl_unseal. iRight.
+    iDestruct (vo_vo_vo2 with "vo vo'") as "$".
+    iApply (proph_eqz_modify with "obs eqz").
   Qed.
 End proph_ag.
