nola/examples/borrow.v
@@ -14,61 +14,69 @@ Section borrow.
   (** Dereference a nested mutable reference *)
   Lemma bor_bor_deref {α β l Φx q} :
     [[{ β ⊑□ α ∗ q.[β] ∗ bor_tok β (∃ l', ▷ l ↦ #l' ∗ cif_bor α (Φx l'))%cif }]]
-      [borrow_wsat bupd_0 ⟦⟧]
+      [borrow_wsat bupd ⟦⟧]
       !#l
     [[{ l', RET #l'; q.[β] ∗ bor_tok β (Φx l') }]].
   Proof.
     iIntros (Ψ) "(#⊑ & [β β'] & b) →Ψ".
-    iMod (bor_tok_open (M:=bupd_0) with "β b") as "/=[o [%l'[>↦ b']]]".
+    iMod (bor_tok_open (M:=bupd) with "β b") as "/=[o [%l'[>↦ b']]]".
     iApply twpw_fupdw_nonval; [done|]. wp_read.
     iMod (lft_sincl_live_acc with "⊑ β'") as (?) "[α →β']".
     rewrite sem_ecustom /=.
-    iMod (bor_tok_reborrow (M:=bupd_0) with "⊑ α b'") as "(α & →b' & b')".
+    iMod (bor_tok_reborrow (M:=bupd) with "⊑ α b'") as "(α & →b' & b')".
     iDestruct ("→β'" with "α") as "β'".
-    iMod (obor_tok_subdiv (M:=bupd_0) [] with "[] o [] [↦ →b']") as "[β _]"=>/=.
+    iMod (obor_tok_subdiv (M:=bupd) [] with "[] o [] [↦ →b']") as "[β _]"=>/=.
     { iApply lft_sincl_refl. } { done. }
     { iIntros "† _ !>". iExists _. iFrame "↦". rewrite sem_ecustom /=.
       by iApply "→b'". }
     iModIntro. iApply "→Ψ". iFrame.
   Qed.
 
-  Context `{!prophGS nsynty Σ, !proph_agG nsynty Σ, !PborCon nsynty CON,
-    !PborSem nsynty JUDG CON Σ}.
-  Implicit Type X : nsynty.
-
-  (** Dereference a nested prophetic mutable reference *)
-  Lemma pbor_pbor_deref {X η ξ α β l Φxx q} {x : X} :
-    [[{ β ⊑□ α ∗ q.[β] ∗
-        pbor_tok β ((x, ξ)' : _ *'ₛ prvarₛ _) η
-          (λ '(x', ξ')', ∃ l', ▷ l ↦ #l' ∗ cif_pbor α x' ξ' (Φxx l'))%cif }]]
-      [borrow_wsat bupd_0 ⟦⟧]
-      !#l
-    [[{ l', RET #l';
-        q.[β] ∗ ∃ ξ' : prvar X,
-          ⟨π, π η = (π ξ', ξ)'⟩ ∗ pbor_tok β x ξ' (Φxx l') }]].
-  Proof.
-    iIntros (Ψ) "(#⊑ & [β β'] & b) →Ψ".
-    iMod (pbor_tok_open (M:=bupd_0) with "β b") as "/=[o[%l'[>↦ b']]]".
-    iApply twpw_fupdw_nonval; [done|]. wp_read.
-    iMod (lft_sincl_live_acc with "⊑ β'") as (?) "[α →β']".
-    rewrite sem_ecustom /=.
-    iMod (pobor_pbor_tok_reborrow (TY:=nsynty) (M:=bupd_0)
-      (λ _, (_,_)' : _ *'ₛ _) with "⊑ o α b' [↦]") as (?) "(β & α & obs & b)".
-    { iIntros "/=% _ ? !>". iExists _. iFrame "↦". by rewrite sem_ecustom /=. }
-    iModIntro. iApply "→Ψ". iDestruct ("→β'" with "α") as "$". iFrame.
-  Qed.
-
   (** Load from an immutable shared borrow *)
   Lemma imbor_load {l α q} {n : Z} :
     [[{ q.[α] ∗ inv_tok nroot (cif_bor α (▷ l ↦ #n)) }]]
-      [inv_wsat ⟦⟧ ∗ borrow_wsat bupd_0 ⟦⟧]
+      [inv_wsat ⟦⟧ ∗ borrow_wsat bupd ⟦⟧]
       !ˢᶜ#l
     [[{ RET #n; q.[α] }]].
   Proof.
     iIntros (Φ) "[α #i] →Φ". iMod (inv_tok_acc with "i") as "/=[b cl]"; [done|].
     rewrite sem_ecustom /=.
-    iMod (bor_tok_open (M:=bupd_0) with "α b") as "/=[o >↦]". wp_read.
-    iMod (obor_tok_close (M:=bupd_0) with "o [↦]") as "[α b]"=>/=; [done|].
+    iMod (bor_tok_open (M:=bupd) with "α b") as "/=[o >↦]". wp_read.
+    iMod (obor_tok_close (M:=bupd) with "o [↦]") as "[α b]"=>/=; [done|].
     iMod ("cl" with "b") as "_". iModIntro. by iApply "→Φ".
+  Qed.
+
+  Context `{!prophGS nsynty Σ, !proph_agG unit nsynty Σ,
+    !PborrowCon unit nsynty CON, !PborCon unit nsynty CON,
+    !PborrowSem unit nsynty JUDG CON Σ, !PborSem unit nsynty JUDG CON Σ}.
+  Implicit Type X : nsynty.
+
+  (** Dereference a nested prophetic mutable reference *)
+  Lemma pbor_pbor_deref {X η α β l Φxx q xxπ} :
+    [[{ β ⊑□ α ∗ q.[β] ∗
+        pbor_tok (X:=X *'ₛ X) β () xxπ η
+          (λ _ xxπ, ∃ l' (xπ : clair _ X) (ξ : prvar X),
+            ⌜xxπ = λ π, (xπ π, π ξ)'⌝ ∗
+            ▷ l ↦ #l' ∗ cif_pbor α () xπ ξ (Φxx l'))%cif }]]
+      [borrow_wsat bupd ⟦⟧]
+      !#l
+    [[{ l', RET #l'; ∃ (xπ : clair _ X) (ξ ξ' : prvar X),
+        ⌜xxπ = λ π, (xπ π, π ξ)'⌝ ∗ ⟨π, π η = (π ξ', π ξ)'⟩ ∗ q.[β] ∗
+        pbor_tok β () xπ ξ' (Φxx l') }]].
+  Proof.
+    iIntros (Ψ) "(#⊑ & [β β'] & b) →Ψ".
+    iMod (pbor_tok_open (M:=bupd) with "β b") as "/=[o big]".
+    iDestruct "big" as (l' xπ ξ ->) "[>↦ b]". rewrite sem_ecustom /=.
+    iApply twpw_fupdw_nonval; [done|]. wp_read.
+    iMod (lft_sincl_live_acc with "⊑ β'") as (?) "[α →β']".
+    iMod (pobor_pbor_tok_reborrow (M:=bupd) (λ π x, (x, π ξ)' : _ *'ₛ _)
+      with "⊑ α o b [↦]") as "(ξ & Φxx & big)"=>/=. { by move=> ????[]. }
+    { iIntros ([]?) "_ ? !>". iExists _, _, _. rewrite sem_ecustom /=.
+      by iFrame. }
+    iMod ("big" $! [Aprvar _ ξ] _ with "[%] [$ξ //]")
+      as (?) "(obs & [ξ _ ] & big)".
+    { move=> ?. apply proph_dep_f. apply: proph_dep_one. }
+    iMod ("big" with "ξ Φxx") as "(β & α & b)". iModIntro. iApply "→Ψ".
+    iDestruct ("→β'" with "α") as "$". by iFrame.
   Qed.
 End borrow.
